Core/Global.lean
@@ -24,7 +24,7 @@ def Global.repr (p : Nat) : (a : Global) -> Std.Format
   ".data " ++ s ++ " : " ++ Kind.repr max_prec K ++ Std.Format.line
       ++ "#𝓋" ++ Std.Format.sbracket (cs.to.fold Std.Format.nil (λ c acc => acc ++ ", " ++ Std.Format.line ++ c))
 
-| odata n K => ".odata " ++ n ++ " " ++ K.repr max_prec
+| .odata n K => ".odata " ++ n ++ " " ++ K.repr max_prec
 | .openm n ty => ".openm " ++ n ++ " : " ++ SpineTy.repr ty
 | .defn n T t => ".defn " ++ n ++ " " ++ T.repr max_prec ++ t.repr max_prec
 | .inst n _ t => "instance " ++ n ++ " " ++  t.repr max_prec
@@ -56,6 +56,23 @@ inductive Entry : Type where
 | openm : String -> SpineTy -> Entry
 | defn : String -> Ty -> Term -> Entry
 | octor : String -> SpineTy -> Entry
+
+def Entry.repr (_ : Nat) : Entry -> Std.Format
+| .data (n := n) x K ctors =>
+  let cs : Fun.Vec Std.Format n := λ i =>
+    let ctorN := (Vec.to ctors i).1
+    let ctorTy := (Vec.to ctors i).2
+    Std.Format.nest 4 <| ctorN ++ SpineTy.repr ctorTy
+  ".data " ++ x ++ " : " ++ Kind.repr max_prec K ++ Std.Format.line
+      ++ "#𝓋" ++ Std.Format.sbracket (cs.to.fold Std.Format.nil (λ c acc => acc ++ ", " ++ Std.Format.line ++ c))
+| .ctor x _ spTy => ".ctor " ++ x ++ " " ++ spTy.repr
+| .odata x K =>  ".odata " ++ x ++ " " ++ K.repr max_prec
+| .openm x spTy => ".openm " ++ x ++ " : " ++ SpineTy.repr spTy
+| .defn x T t => ".defn " ++ x ++ " " ++ T.repr max_prec ++ t.repr max_prec
+| .octor x spTy => ".octor " ++ x ++ SpineTy.repr spTy
+
+instance instRepr_Entry : Repr Entry where
+  reprPrec e p := Entry.repr p e
 
 def Entry.name : Entry -> String
 | data x _ _ => x
