Core/Infer/TypeSound.lean
@@ -3,12 +3,62 @@ import Core.Infer.KindSound
 import Core.Infer.«Type»
 import Core.Ty
 import Core.Typing
+import LeanSubst
 
 import Core.Vec
 import Lilac
 open Lilac
+open LeanSubst
+
 
 namespace Core
+
+theorem pattern_binders_sound :
+  pattern_binders G Δ m Ts p = some Γ ->
+  PatternBinders G Δ m Ts p Γ := by
+intro h
+induction m generalizing Γ <;> simp at *
+case _ =>
+  cases Ts; cases p; cases h
+  apply PatternBinders.zero
+case _ n ih =>
+  cases Ts; case _ T S =>
+  cases p; case _ p ps' =>
+  unfold pattern_binders at h;
+  simp at h;
+  rw[Option.bind_eq_some_iff] at h; rcases h with ⟨Γ', h2, h⟩
+  rw[Option.bind_eq_some_iff] at h; rcases h with ⟨h3, h4, h⟩
+  simp at h; rcases h with ⟨h5, h⟩
+  rw[Option.bind_eq_some_iff] at h; rcases h with ⟨Ks, h6, h⟩; simp at h
+  rcases h with ⟨h7, h8, h9⟩
+  replace ih := @ih _ _ Γ' h2
+  replace h6 := Vec.seq_sound h6
+  simp only [<-h5.2] at Ks
+  simp [SpineTy] at h3;
+  let Ts := h3.2.2.2.fst
+  let Ts'' := Vec.map (fun T => T[Sequ.append_vec (Vec.map LeanSubst.su p.2.2.fst) +0:_]) Ts
+  let R := h3.2.2.2.2
+  let As := p.2.2.fst
+  rw[<-h5.2] at As
+  let R' := R[Sequ.append_vec (Vec.map su As) +0:Ty]
+  generalize c_def : p.fst = c at *
+  let na := p.2.fst
+  let na' := h3.1
+  let nb := p.2.2.2
+  let nb' := h3.2.2.1
+  let h := @PatternBinders.succ G Δ h3.snd.snd.1 c h3.1 Ks (S := S) (p := ps') (ℓ := Γ') (R := R) (As := As) (R' := R') (Ts := Ts) (Ts' := Ts'') n
+    (by rw[h4]; simp; sorry)
+    (by intro i; rw[h5.2] at i; replace h6 := h6 i; sorry)
+    (by unfold Ts''; sorry)
+    (by unfold R'; rfl) ih
+  subst h9; subst h8;
+  simp at h; unfold R' at h; unfold R at h
+
+  sorry
+
+
+
+
 
 theorem infer_type_sound :
   ⊢ G ->
